Adding containers for read_option.

lib/Heap.v
@@ -3,32 +3,157 @@
 
 From Coq Require Import FSets.FMapAVL.
 From Lib Require Import LibExec.
-From TLC Require Export LibContainer.
+From TLC Require Export LibTactics LibReflect LibContainer.
 
-Class Comparable_lt T := {
-    lt : T -> T -> bool ;
-    lt_trans : forall x y z : T, lt x y -> lt y z -> lt x z ;
-    lt_not_eq : forall x y : T, lt x y -> ~ x = y
+
+(** * Addition to LibContainer about read_option **)
+
+(** ** Definitions **)
+
+Class BagReadOption A B T := { read_option : T -> A -> option B }.
+
+Class BagInDec A T := {
+    bag_in :> BagIn A T ;
+    bag_in_dec :> forall a (t : T), Decidable (a \in t)
   }.
 
-Section Heap.
+(** ** Properties **)
 
-Variable K : Type.
-Hypothesis K_comparable : Comparable K.
+Section Properties.
 
-Module K_OrderedType : OrderedType.OrderedType. (* Doesn’t work: once module-based, one has to stay module based. *)
+Context {A B T D : Type}
+  {BI : BagIn A T} {BE : BagEmpty T} {BR : BagRead A B T} {BRO : BagReadOption A B T} {BD : BagDom T D}.
 
-   Parameter eq : t -> t -> Prop.
-   Parameter lt : t -> t -> Prop.
-   Parameter eq_refl : forall x : t, eq x x.
-   Parameter eq_sym : forall x y : t, eq x y -> eq y x.
-   Parameter eq_trans : forall x y z : t, eq x y -> eq y z -> eq x z.
-   Parameter lt_trans : forall x y z : t, lt x y -> lt y z -> lt x z.
-   Parameter lt_not_eq : forall x y : t, lt x y -> ~ eq x y.
-   Parameter compare : forall x y : t, OrderedType.Compare lt eq x y.
-   Parameter eq_dec : forall x y : t, {eq x y} + {~ eq x y}.
+Class ReadOption_In_eq := {
+    read_option_in_eq : forall a t, a \notin t -> read_option t a = None
+  }.
 
-Definition Tree X :=
-  FMapAVL.Make(X).
+Class ReadOption_Read_eq := {
+    read_option_read_eq : forall a b t, read_option a t = Some b -> read a t = b
+  }.
 
-Definition heap K V := FMapAVL .tree
+End Properties.
+
+(** ** Conversions **)
+
+Definition ReadOptionToRead A B T `{BagReadOption A B T} `{Inhab B} : BagRead A B T := {|
+    read t a :=
+      match read_option t a with
+      | None => arbitrary
+      | Some b => b
+      end
+  |}.
+
+Instance ReadOptionToRead_ReadOption_Read_eq : forall A B T `{BagReadOption A B T} `{Inhab B},
+  ReadOption_Read_eq (BR := ReadOptionToRead A B T).
+Proof.
+  constructors. introv E. simpl. rewrite~ E.
+Qed.
+
+Definition ReadOptionToIn A B T `{BagReadOption A B T} : BagIn A T := {|
+    is_in a t :=
+      match read_option t a with
+      | None => False
+      | Some _ => True
+      end
+  |}.
+
+Instance ReadOptionToIn_ReadOption_In_eq : forall A B T `{BagReadOption A B T},
+  ReadOption_In_eq (BI := ReadOptionToIn A B T).
+Proof.
+  constructors. unfold notin. simpl. introv. destruct* read_option.
+Qed.
+
+Definition ReadToReadOption A B T `{BagRead A B T} `{BagInDec A T} : BagReadOption A B T := {|
+    read_option t a :=
+      ifb a \in t then Some (read t a) else None
+  |}.
+
+Instance ReadToReadOption_ReadOption_Read_eq : forall A B T `{BagRead A B T} `{BagInDec A T},
+  ReadOption_Read_eq (BRO := ReadToReadOption A B T).
+Proof.
+  constructors. simpl. introv E. cases_if; inverts~ E.
+Qed.
+
+Instance ReadToReadOption_ReadOption_In_eq : forall A B T `{BagRead A B T} `{BagInDec A T},
+  ReadOption_In_eq (BRO := ReadToReadOption A B T).
+Proof.
+  constructors. simpl. introv E. cases_if as D; autos~.
+  rewrite decide_spec in D. rew_istrue in D. false~ E.
+Qed.
+
+
+(** * Instanciation of heaps **)
+
+Module HeapFromOrdered (X : OrderedType.OrderedType).
+
+Export X.
+
+Definition K := t.
+
+Module Export Tree := FMapAVL.Make(X).
+
+Instance read_option_inst V : BagReadOption K V (t V) := {|
+    read_option t a := find a t
+  |}.
+
+Instance read_inst V `{Inhab V} : BagRead K V (t V) :=
+  ReadOptionToRead K V _.
+
+Instance in_inst V : BagIn K (t V) :=
+  ReadOptionToIn K V _.
+
+End HeapFromOrdered.
+
+
+(** * Building [OrderedType.OrderedType] from TLC. **)
+
+Class Comparable_lt T := Build_Comparable_lt {
+    lt : T -> T -> bool ;
+    lt_trans : forall x y z : T, lt x y -> lt y z -> lt x z ;
+    lt_not_eq : forall x y : T, lt x y -> ~ x = y ;
+    lt_total : forall x y, lt x y \/ x = y \/ lt y x
+  }.
+
+Module Type ComparableLt.
+
+Parameter t : Type.
+
+Parameter comparable : Comparable t.
+Parameter comparable_lt : Comparable_lt t.
+
+End ComparableLt.
+
+Module OrderedTypeFromComparable (X : ComparableLt) : OrderedType.OrderedType.
+
+Include X.
+
+Definition eq := @eq t.
+Definition lt a b : Prop := @lt t comparable_lt a b.
+
+Definition eq_refl := @eq_refl t.
+Definition eq_sym := @eq_sym t.
+Definition eq_trans x y z := @eq_trans t y x z.
+
+Definition lt_trans := @lt_trans t comparable_lt.
+Definition lt_not_eq := @lt_not_eq t comparable_lt.
+
+Lemma compare : forall x y : t, OrderedType.Compare lt eq x y.
+Proof.
+  introv. destruct (@Heap.lt t comparable_lt x y) eqn: L.
+  - applys~ OrderedType.LT.
+  - destruct (@decide (x = y) (@LibExec.comparable _ comparable _ _)) eqn: E.
+    + rewrite decide_spec in E. rew_bool_eq in E. applys~ OrderedType.EQ.
+    + rewrite decide_spec in E. rew_bool_eq in *. applys OrderedType.GT.
+      destruct (@lt_total _ comparable_lt x y) as [H|[H|H]]; tryfalse.
+      autos~.
+Defined.
+
+Lemma eq_dec : forall x y : t, {eq x y} + {~ eq x y}.
+Proof.
+  introv. applys~ decidable_sumbool comparable.
+Defined.
+
+End OrderedTypeFromComparable.
+
+Module Heap (X : ComparableLt) := HeapFromOrdered (OrderedTypeFromComparable (X)).
